Weidenbach_Book/IsaSAT_Propagate_Conflict_SML.thy
@@ -12,10 +12,29 @@ sepref_definition length_ll_fs_heur_code
 
 declare length_ll_fs_heur_code.refine[sepref_fr_rules]
 
+definition length_aa64_u32 :: \<open>('a::heap array_list64) array \<Rightarrow> uint32 \<Rightarrow> uint64 Heap\<close> where
+  \<open>length_aa64_u32 xs i = do {
+     x \<leftarrow> nth_u_code xs i;
+    arl64_length x}\<close>
+
+lemma length_aa64_rule[sep_heap_rules]:
+    \<open>b < length xs \<Longrightarrow> (b', b) \<in> uint32_nat_rel \<Longrightarrow> <arrayO_assn (arl64_assn R) xs a> length_aa64_u32 a b'
+    <\<lambda>r. arrayO_assn (arl64_assn R) xs a * \<up> (nat_of_uint64 r = length_ll xs b)>\<^sub>t\<close>
+  unfolding length_aa64_u32_def nth_u_code_def Array.nth'_def
+  apply (sep_auto simp flip: nat_of_uint32_code simp: br_def uint32_nat_rel_def length_ll_def)
+  apply (subst arrayO_except_assn_array0_index[symmetric, of b])
+  apply (simp add: nat_of_uint32_code br_def uint32_nat_rel_def)
+  apply (sep_auto simp: arrayO_except_assn_def)
+  done
+
+lemma length_aa64_u32_hnr[sepref_fr_rules]: \<open>(uncurry length_aa64_u32, uncurry (RETURN \<circ>\<circ> length_ll)) \<in>
+     [\<lambda>(xs, i). i < length xs]\<^sub>a (arrayO_assn (arl64_assn R))\<^sup>k *\<^sub>a uint32_nat_assn\<^sup>k \<rightarrow> uint64_nat_assn\<close>
+  by sepref_to_hoare (sep_auto simp: uint32_nat_rel_def br_def uint64_nat_rel_def)
+
 sepref_definition length_ll_fs_heur_fast_code
   is \<open>uncurry (RETURN oo length_ll_fs_heur)\<close>
   :: \<open>[\<lambda>(S, L). nat_of_lit L < length (get_watched_wl_heur S)]\<^sub>a
-      isasat_bounded_assn\<^sup>k *\<^sub>a unat_lit_assn\<^sup>k \<rightarrow>nat_assn\<close>
+      isasat_bounded_assn\<^sup>k *\<^sub>a unat_lit_assn\<^sup>k \<rightarrow> uint64_nat_assn\<close>
   unfolding length_ll_fs_heur_alt_def get_watched_wl_heur_def isasat_bounded_assn_def
     length_ll_def[symmetric]
   supply [[goals_limit=1]] length_ll_def[simp]
@@ -54,7 +73,6 @@ sepref_definition unit_propagation_inner_loop_wl_loop_D_fast
   unfolding delete_index_and_swap_update_def[symmetric] append_update_def[symmetric]
     is_None_def[symmetric] get_conflict_wl_is_None_heur_alt_def[symmetric]
     length_ll_fs_def[symmetric] zero_uint64_nat_def[symmetric]
-  apply (rewrite at \<open>let _ = \<hole> in _\<close> uint64_of_nat_conv_def[symmetric])
   supply [[goals_limit=1]] unit_propagation_inner_loop_wl_loop_D_heur_fast[intro]
   by sepref
 
@@ -74,7 +92,22 @@ sepref_definition cut_watch_list_heur2_code
 
 declare cut_watch_list_heur2_code.refine[sepref_fr_rules]
 
+definition (in -) shorten_take_aa64_u32 where
+  \<open>shorten_take_aa64_u32 L j W =  do {
+      (a, n) \<leftarrow> nth_u_code W L;
+      Array_upd_u L (a, j) W
+    }\<close>
 
+lemma shorten_take_aa_hnr[sepref_fr_rules]:
+  \<open>(uncurry2 shorten_take_aa64_u32, uncurry2 (RETURN ooo shorten_take_ll)) \<in>
+     [\<lambda>((L, j), W). j \<le> length (W ! L) \<and> L < length W]\<^sub>a
+    uint32_nat_assn\<^sup>k *\<^sub>a uint64_nat_assn\<^sup>k *\<^sub>a (arrayO_assn (arl64_assn R))\<^sup>d \<rightarrow> arrayO_assn (arl64_assn R)\<close>
+  unfolding shorten_take_aa64_u32_def shorten_take_ll_def nth_u_code_def Array.nth'_def
+    comp_def nat_of_uint32_code[symmetric] Array_upd_u_def
+  by sepref_to_hoare (sep_auto simp: uint32_nat_rel_def br_def uint64_nat_rel_def)
+
+find_theorems shorten_take_ll arl64_assn
+thm shorten_take_aa_hnr
 sepref_definition cut_watch_list_heur2_fast_code
   is \<open>uncurry3 cut_watch_list_heur2\<close>
   :: \<open>[\<lambda>(((j, w), L), S). length (watched_by_int S L) \<le> uint64_max-4]\<^sub>a
@@ -84,7 +117,6 @@ sepref_definition cut_watch_list_heur2_fast_code
   unfolding cut_watch_list_heur2_def isasat_bounded_assn_def length_ll_def[symmetric]
   update_ll_def[symmetric] nth_rll_def[symmetric] shorten_take_ll_def[symmetric]
   one_uint64_nat_def[symmetric] length_rll_def[symmetric]
-  apply (rewrite in \<open>shorten_take_ll _ \<hole> _\<close> nat_of_uint64_conv_def[symmetric])
   by sepref
 
 declare cut_watch_list_heur2_fast_code.refine[sepref_fr_rules]
@@ -108,7 +140,7 @@ sepref_definition unit_propagation_inner_loop_wl_D_fast_code
 
 declare unit_propagation_inner_loop_wl_D_fast_code.refine[sepref_fr_rules]
 
-  
+
 sepref_definition select_and_remove_from_literals_to_update_wl_code
   is \<open>select_and_remove_from_literals_to_update_wl_heur\<close>
   :: \<open>isasat_unbounded_assn\<^sup>d \<rightarrow>\<^sub>a isasat_unbounded_assn *a unat_lit_assn\<close>
